theories/cap_lang.v
@@ -689,9 +689,9 @@ Section opsem.
        |>> updatePC
 
     (* enclave deinitialization *)
-  | EDeInit rs =>
-      wσ   ← (reg φ) !! rs; (* σ should be a seal/unseal pair *)
-      '(p,σb,σe,σa) ← get_sealing_cap wσ;
+  | EDeInit r =>
+      wr   ← (reg φ) !! r; (* σ should be a seal/unseal pair *)
+      '(p,σb,σe,σa) ← get_sealing_cap wr;
       when ((bool_decide (p = (true,true))) && (σe =? σb^+2)%ot) then
       tid ← tid_of_otype σb;
 
